rename in coq workloads

workloads/Coq/RBT/Strategies/BespokeGenerator.v
@@ -1,4 +1,6 @@
 
+
+
 Require Import ZArith.
 From QuickChick Require Import QuickChick.
 From ExtLib Require Import Monad.
@@ -9,51 +11,68 @@ From Coq Require Import List.
 Import ListNotations.
 
 
-From RedBlack Require Import Impl Spec.
+From RBT Require Import Impl Spec.
+
+Open Scope Z_scope.
+
+Fixpoint genTree (lo hi : Z) (c : Color)  (f: nat) (h : nat) : G (option Tree) 
+:=
+if lo >? hi then ret None else
+match f with
+| S f' =>
+  match h, c with
+  | O, R => ret (Some E)
+  | O, B => oneOf [ ret (Some E)
+                        ; k <- choose (lo, hi) ;;
+                          v <- arbitrary ;;
+                          ret (Some (T R E k v E))]
+  | S h', R =>
+      let margin := (2^(2*(Z.of_nat h) - 1) - 1) in
+      if (lo + margin >? hi - margin) then  ret None else
+      c' <- ret B ;;
+      k <- choose (lo + margin, hi - margin) ;;
+      v <- arbitrary ;;
+      l <- genTree lo (k - 1)  B f' h' ;;
+      r <- genTree (k + 1) hi  B f' h' ;;
+       match l, r with
+      | Some tl, Some tr => ret (Some (T c' tl k v tr))
+      | _, _ => ret None
+      end
+          
+  | S h', B =>
+      let margin := (2^(2*(Z.of_nat h)) - 1) in
+      if (lo + margin >? hi - margin) then ret None else
+      c' <- arbitrary ;;
+      k <- choose (lo + margin, hi - margin) ;;
+      v <- arbitrary ;;
+      let h'' := match c' with R => h | B => h' end in
+      l <- genTree lo (k - 1) c' f' h'' ;;
+      r <- genTree (k + 1) hi c' f' h'' ;;
+      match l, r with
+      | Some tl, Some tr => ret (Some (T c' tl k v tr))
+      | _, _ => ret None
+      end
+  end
+| _ => ret None
+end.
+
+Axiom fuel : nat. Extract Constant fuel => "10000".
+
+Global Instance genTreeSized : GenSized (option Tree) :=
+{| arbitrarySized x := 
+    let y := Nat.min x 2 in
+      genTree 0 (2^(Z.of_nat(y)*2)) R fuel y |}.
 
 
-
-Local Open Scope Z_scope.
-
-
-Inductive between : Z -> Z -> Z -> Prop :=
-| between_n : forall n m, Z.le n m -> between n (n + 1) (m + 2)
-| between_S : forall n m o, between n m o -> between n (m + 1) (o + 1).
-
-Inductive red_black_bst : Color -> nat -> Z -> Z -> Tree -> Prop :=
-    rbt_leafbh_leafbst_leaf : forall (lo hi : Z) (c : Color),
-                              red_black_bst c 1 lo hi E
-  | rbt_black_nodebh_black_nodebst_node : forall (lo hi x y: Z)
-                                            (l r : Tree) (h : nat)
-                                            (c1 c2 : Color),
-                                          between lo x hi ->
-                                          red_black_bst c1 h lo x l ->
-                                          red_black_bst c2 h x hi r ->
-                                          red_black_bst B (S h) lo hi (T B l x y r)
-  | rbt_red_nodebh_red_nodebst_node : forall (lo hi x y: Z) (l r : Tree) (h : nat),
-                                      between lo x hi ->
-                                      red_black_bst B h lo x l ->
-                                      red_black_bst B h x hi r ->
-                                      red_black_bst R h lo hi (T R l x y r).
-
-
-#[local] Instance gen_between (lo hi : Z) :
-GenSizedSuchThat _ (fun x => between lo x hi) :=
-{| arbitrarySizeST := fun n =>
-                        if Z.leb 2 (hi - lo) then
-                          bindGen (choose (lo+1,hi-1)%Z) (fun x => ret (Some x))
-                        else ret None
-|}%nat.
-
-Derive ArbitrarySizedSuchThat for (fun t => red_black_bst c h lo hi t).
-
-Definition gRbt := 
-    (@arbitrarySizeST _ (fun t => red_black_bst B 3 0 100 t) _ 10).
+Definition gSized := 
+    x <- choose (0, 3)%nat;;
+    genTree 0 (2^(Z.of_nat(x)*2)) R fuel x
+.
 
 (* --------------------- Tests --------------------- *)
 
 Definition test_prop_InsertValid :=  
-    forAllMaybe gRbt (fun t =>    
+    forAllMaybe gSized (fun t =>    
     forAll arbitrary (fun k =>
     forAll arbitrary (fun v =>
         (prop_InsertValid t k v)))).
@@ -61,14 +80,14 @@ Definition test_prop_InsertValid :=
 (*! QuickChick test_prop_InsertValid. *)
 
 Definition test_prop_DeleteValid :=  
-    forAllMaybe gRbt (fun t =>    
+    forAllMaybe gSized (fun t =>    
     forAll arbitrary (fun k =>
         prop_DeleteValid t k)).
 
 (*! QuickChick test_prop_DeleteValid. *)
 
 Definition test_prop_InsertPost :=  
-    forAllMaybe gRbt (fun t =>    
+    forAllMaybe gSized (fun t =>    
     forAll arbitrary (fun k =>
     forAll arbitrary (fun k' =>
      forAll arbitrary (fun v =>
@@ -77,7 +96,7 @@ Definition test_prop_InsertPost :=
 (*! QuickChick test_prop_InsertPost. *)
 
 Definition test_prop_DeletePost := 
-    forAllMaybe gRbt (fun t =>    
+    forAllMaybe gSized (fun t =>    
     forAll arbitrary (fun k =>
     forAll arbitrary (fun k' =>
         prop_DeletePost t k k'))).
@@ -85,7 +104,7 @@ Definition test_prop_DeletePost :=
 (*! QuickChick test_prop_DeletePost. *)
     
 Definition test_prop_InsertModel :=  
-    forAllMaybe gRbt (fun t =>    
+    forAllMaybe gSized (fun t =>    
     forAll arbitrary (fun k =>
     forAll arbitrary (fun v =>
         prop_InsertModel t k v))).
@@ -93,14 +112,14 @@ Definition test_prop_InsertModel :=
 (*! QuickChick test_prop_InsertModel. *)
     
 Definition test_prop_DeleteModel :=  
-    forAllMaybe gRbt (fun t =>    
+    forAllMaybe gSized (fun t =>    
     forAll arbitrary (fun k =>
             prop_DeleteModel t k)).
 
 (*! QuickChick test_prop_DeleteModel. *)
 
 Definition test_prop_InsertInsert :=  
-    forAllMaybe gRbt (fun t =>    
+    forAllMaybe gSized (fun t =>    
     forAll arbitrary (fun k =>
     forAll arbitrary (fun k' =>
     forAll arbitrary (fun v =>
@@ -110,7 +129,7 @@ Definition test_prop_InsertInsert :=
 (*! QuickChick test_prop_InsertInsert. *)
     
 Definition test_prop_InsertDelete := 
-    forAllMaybe gRbt (fun t =>    
+    forAllMaybe gSized (fun t =>    
     forAll arbitrary (fun k =>
     forAll arbitrary (fun k' =>
     forAll arbitrary (fun v =>
@@ -119,7 +138,7 @@ Definition test_prop_InsertDelete :=
 (*! QuickChick test_prop_InsertDelete. *)
     
 Definition test_prop_DeleteInsert := 
-    forAllMaybe gRbt (fun t =>    
+    forAllMaybe gSized (fun t =>    
     forAll arbitrary (fun k =>
     forAll arbitrary (fun k' =>
     forAll arbitrary (fun v' =>
@@ -128,7 +147,7 @@ Definition test_prop_DeleteInsert :=
 (*! QuickChick test_prop_DeleteInsert. *)
     
 Definition test_prop_DeleteDelete :=  
-    forAllMaybe gRbt (fun t =>    
+    forAllMaybe gSized (fun t =>    
     forAll arbitrary (fun k =>
     forAll arbitrary (fun k' =>
         prop_DeleteDelete t k k'))).
