workloads/Coq/RBT/Runners/HandwrittenNaive_test_runner.v
@@ -1,4 +1,4 @@
-From RedBlack Require Import RookieGenerator.
+From RBT Require Import HandwrittenNaive.
 From QuickChick Require Import QuickChick.
 Set Warnings "-extraction-opaque-accessed,-extraction".
 Axiom num_tests : nat. Extract Constant num_tests => "max_int".
@@ -30,4 +30,4 @@ let () =
   Sys.argv.(1) |> qctest_map
 ".
 
-Extraction "RookieGenerator_test_runner.ml" qctest_test_prop_InsertValid qctest_test_prop_DeleteValid qctest_test_prop_InsertPost qctest_test_prop_DeletePost qctest_test_prop_InsertModel qctest_test_prop_DeleteModel qctest_test_prop_InsertInsert qctest_test_prop_InsertDelete qctest_test_prop_DeleteInsert qctest_test_prop_DeleteDelete qctest_map.
+Extraction "HandwrittenNaive_test_runner.ml" qctest_test_prop_InsertValid qctest_test_prop_DeleteValid qctest_test_prop_InsertPost qctest_test_prop_DeletePost qctest_test_prop_InsertModel qctest_test_prop_DeleteModel qctest_test_prop_InsertInsert qctest_test_prop_InsertDelete qctest_test_prop_DeleteInsert qctest_test_prop_DeleteDelete qctest_map.
