workloads/Coq/RBT/Runners/TypeBasedFuzzer_test_runner.v
@@ -1,4 +1,4 @@
-From RedBlack Require Import TypeBasedFuzzer.
+From RBT Require Import TypeBasedFuzzer.
 From QuickChick Require Import QuickChick.
 Set Warnings "-extraction-opaque-accessed,-extraction".
 Definition qctest_test_prop_InsertValid := (fun _ : unit => print_extracted_coq_string ("[|{" ++ show (withTime (fun tt => (test_prop_InsertValid_fuzzer tt))) ++ "}|]")).
